\documentclass[11pt]{article}
\usepackage{amsmath,amssymb,amsfonts}


\begin{document}

(a)  $ \cos (\alpha - \beta) = \cos\alpha \cos \beta + \sin \alpha \sin \beta) $ \\

From the law of cosines, \\

$
| \vec{a} - \vec{b} |^2 = | \vec{a} |^2 + | \vec{b} |^2 - 2 | \vec{a} | | \vec{b} | \cos (\alpha - \beta) 
$
\\

$
\begin{array}{rcl}
| \vec{a} - \vec{b} |^2  & = & (a \cos \alpha - b \cos \beta)^2 - (a \sin \alpha - b \sin \beta)^2 \\
\\
& = & ( a^2\cos^2\alpha - 2ab \cos\alpha\cos\beta + b^2\cos^2\beta) + (a^2\sin\alpha - 2ab\sin\alpha\sin\beta + b^2\sin^2\beta) \\
\\
& = & a^2 + b^2 - 2ab(\cos\alpha\cos\beta+\sin\alpha\sin\beta)

\end{array}
$

\\

$
|\vec{a}|^2+|\vec{b}|^2-2|\vec{a}||\vec{b}|\cos(\alpha-\beta) = a^2 + b^2 - 2ab\cos(\alpha-\beta)
$
\\

$
\therefore \cos (\alpha - \beta) = \cos\alpha \cos \beta - \sin \alpha \sin \beta)
$
\\

(b)  $ \sin (\alpha - \beta) = \sin\alpha \cos \beta - \cos \alpha \sin \beta $ \\

From the Pythagorean identity, \\

$
\sin^2(\alpha-\beta)+\cos^2(\alpha-\beta) = 1
$
\\ 

$
\begin{array}{rcl}
\sin(\alpha-\beta) & = & \sqrt{1-\cos^2(\alpha-\beta)} \\
\\
& = & \sqrt{1-(\cos\alpha\cos\beta+\sin\alpha\sin\beta)^2} \\
\\
& = & \sqrt{1-(\cos^2\alpha\cos^2\beta+2\cos\alpha\cos\beta\sin\alpha\sin\beta+\sin^2\alpha\sin^2\beta)} \\
\\
& = & \sqrt{1-\{\cos^2\alpha(1-\sin^2\beta)+2\cos\alpha\cos\beta\sin\alpha\sin\beta+\sin^2\alpha(1-\cos^2\beta)\}} \\
\\
& = & \sqrt{1-(\cos^2-\cos^2\sin^2\beta+2\cos\alpha\cos\beta\sin\alpha\sin\beta+\sin^2\alpha-\sin^2\alpha\cos^2\beta)} \\
\\
& = & \sqrt{\cos^2\sin^2\beta-2\cos\alpha\cos\beta\sin\alpha\sin\beta+\sin^2\alpha\cos^2\beta} \\
\\
& = & \sqrt{(\cos\alpha\sin\beta-\sin\alpha\cos\beta)^2} \\
\\
& = & \cos\alpha\sin\beta-\sin\alpha\cos\beta
\end{array}
$
\\

$
\therefore \sin(\alpha-\beta) = \cos\alpha\sin\beta-\sin\alpha\cos\beta
$

\end{document}
