\documentclass[a4paper]{article}

\usepackage[paperwidth=21cm, paperheight=16cm, margin=0.2cm]{geometry}
\usepackage{amsmath}
\usepackage{amssymb}
\usepackage{amsfonts}
\usepackage{diagbox}
\usepackage{graphicx}
\usepackage[makeroom]{cancel}
\usepackage{xcolor}
\usepackage{verbatim}

\usepackage{titlesec}
\titleformat*{\section}{\Huge\bfseries}
\titlespacing*{\section}
{0pt}{5.5ex plus 1ex minus .2ex}{4.3ex plus .2ex}
\titleformat*{\subsection}{\LARGE\bfseries}
\titlespacing*{\subsection}
{0pt}{5.5ex plus 1ex minus .2ex}{4.3ex plus .2ex}


\begin{document}
\Large

\section{Equation Array (Left)}

\begin{comment}
$\begin{array}{rcl}
	
\end{array}
\end{comment}

$\begin{array}{rcl}
	| \vec{a} - \vec{b} |^2  & = & (a \cos \alpha - b \cos \beta)^2 - (a \sin \alpha - b \sin \beta)^2 \\
\\
	& = & ( a^2\cos^2\alpha - 2ab \cos\alpha\cos\beta + b^2\cos^2\beta) + (a^2\sin\alpha - 2ab\sin\alpha\sin\beta + b^2\sin^2\beta) \\
\\
	& = & a^2 + b^2 - 2ab(\cos\alpha\cos\beta+\sin\alpha\sin\beta
\end{array}
$\\\\

$
\begin{array}{rcl}
\sin(\alpha-\beta) & = & \sqrt{1-\cos^2(\alpha-\beta)} \\\\
& = & \sqrt{1-(\cos\alpha\cos\beta+\sin\alpha\sin\beta)^2} \\\\
& = & \sqrt{1-(\cos^2\alpha\cos^2\beta+2\cos\alpha\cos\beta\sin\alpha\sin\beta+\sin^2\alpha\sin^2\beta)} \\\\
& = & \sqrt{1-\{\cos^2\alpha(1-\sin^2\beta)+2\cos\alpha\cos\beta\sin\alpha\sin\beta+\sin^2\alpha(1-\cos^2\beta)\}} \\\\
& = & \sqrt{1-(\cos^2\alpha-\cos^2\alpha\sin^2\beta+2\cos\alpha\cos\beta\sin\alpha\sin\beta+\sin^2\alpha-\sin^2\alpha\cos^2\beta)} \\\\
& = & \sqrt{\cos^2\alpha\sin^2\beta-2\cos\alpha\cos\beta\sin\alpha\sin\beta+\sin^2\alpha\cos^2\beta} \\\\
& = & \sqrt{(\cos\alpha\sin\beta-\sin\alpha\cos\beta)^2} \\\\
& = & \cos\alpha\sin\beta-\sin\alpha\cos\beta
\end{array}	
$
\\\\

\section{Equation Array (Center)}

\begin{comment}
\begin{eqnarray*}
	
\end{eqnarray*}
\end{comment}

\begin{eqnarray*}
	\sum_{j,k} \epsilon_{ijk} \ \epsilon_{ljk} & = & \epsilon_{i12} \ \epsilon_{l12} + \epsilon_{i13} \ \epsilon_{l13} + \epsilon_{i21} \ \epsilon_{l21} + \epsilon_{i23} \ \epsilon_{l23} + \epsilon_{i31} \ \epsilon_{i31} + \epsilon_{i32} \ \epsilon_{l32}\\
	& = & 0\cdot0 + 0\cdot(-1) + 0\cdot0 + 1\cdot0 + 0\cdot1 + (-1)\cdot0 \quad = 0 \text{\qquad when $i=1,\ l=2$} \\\\
	& = & 0\cdot(-1) + 0\cdot0 + 0\cdot(-1) + 1\cdot0 + 0\cdot0 + (-1)\cdot0 \quad = 0 \text{\qquad when $i=1, \ l=3$} \\\\
	& = & 0\cdot0 + (-1)\cdot0 + 0\cdot0 + 0\cdot1 + 1\cdot0 + 0\cdot(-1) \quad = 0 \text{\qquad when $i=2,\ l=1$} \\\\
	& = & 0\cdot1 + (-1)\cdot0 + 0\cdot(-1) + 0\cdot0 + 1\cdot0 + 1\cdot0 \quad = 0 \text{\qquad when $i=2,\ l=3$} \\\\
	& = & (-1)\cdot0 + 0\cdot0 + (-1)\cdot0 + 0\cdot1 + 0\cdot0 + 0\cdot(-1) \quad = 0 \text{\qquad when $i=3,\ l=1$} \\\\
	& = & (-1)\cdot0 + 0\cdot(-1) + (-1)\cdot0 + 0\cdot0 + 0\cdot1 + 0\cdot0 \quad = 0 \text{\qquad when $i=3,\ l=2$}
\end{eqnarray*}

\end{document}